WIP

src/NoSync2Stutter.v
@@ -32,8 +32,6 @@ Section GENORDER.
   Let srcE := ((@eventE _ident_src +' cE) +' sE state_src).
   Let tgtE := ((@eventE _ident_tgt +' cE) +' sE state_tgt).
 
-  Variable wf_stt: WF.
-
   Let shared :=
     (TIdSet.t *
        (@imap ident_src wf_src) *
@@ -46,153 +44,219 @@ Section GENORDER.
 
   Variable I: shared_rel.
 
-  Variant __geno
+  Let A R0 R1 := (bool * bool * URA.car * (itree srcE R0) * (itree tgtE R1) * shared)%type.
+  Let wf_ot {R0 R1} := @ord_tree_WF (A R0 R1).
+  Let wf_stt {R0 R1} := sum_WF (@wf_ot R0 R1) (@wf_ot R0 R1).
+
+  Variant _geno
           (tid: thread_id)
-          (* (geno: forall R_src R_tgt (RR: R_src -> R_tgt -> URA.car -> shared_rel), bool -> bool -> URA.car -> (wf_stt.(T) * itree srcE R_src) -> itree tgtE R_tgt -> shared_rel) *)
-          (_geno: forall R_src R_tgt (RR: R_src -> R_tgt -> URA.car -> shared_rel),bool -> bool -> URA.car -> (wf_stt.(T) * itree srcE R_src) -> itree tgtE R_tgt -> shared_rel)
+          (geno: forall R_src R_tgt (RR: R_src -> R_tgt -> URA.car -> shared_rel), bool -> bool -> URA.car -> ((@wf_stt R_src R_tgt).(T) * itree srcE R_src) -> itree tgtE R_tgt -> shared_rel)
           R_src R_tgt (RR: R_src -> R_tgt -> URA.car -> shared_rel)
     :
-    bool -> bool -> URA.car -> (wf_stt.(T) * itree srcE R_src) -> itree tgtE R_tgt -> shared_rel :=
+    bool -> bool -> URA.car -> ((@wf_stt R_src R_tgt).(T) * itree srcE R_src) -> itree tgtE R_tgt -> shared_rel :=
   | geno_ret
-      f_src f_tgt r_ctx o o0
+      f_src f_tgt r_ctx o
       ths im_src im_tgt st_src st_tgt r_shared
       r_src r_tgt
-      (LT: wf_stt.(lt) o0 o)
+      ol or ol0 or0
+      (FL: f_src = false -> o = inl ol)
+      (TR: f_src = true -> o = inr or)
+      (LTL: wf_ot.(lt) ol0 ol)
+      (LTR: wf_ot.(lt) or0 or)
       (GENO: RR r_src r_tgt r_ctx (ths, im_src, im_tgt, st_src, st_tgt, r_shared))
     :
-    __geno tid geno _geno RR f_src f_tgt r_ctx (o, Ret r_src) (Ret r_tgt) (ths, im_src, im_tgt, st_src, st_tgt, r_shared)
+    _geno tid geno RR f_src f_tgt r_ctx (o, Ret r_src) (Ret r_tgt) (ths, im_src, im_tgt, st_src, st_tgt, r_shared)
 
   | geno_tauL
       f_src f_tgt r_ctx o
       ths im_src im_tgt st_src st_tgt r_shared
       itr_src itr_tgt
-      (GENO: _geno _ _ RR true f_tgt r_ctx (o, itr_src) itr_tgt (ths, im_src, im_tgt, st_src, st_tgt, r_shared))
+      ol or
+      (FL: f_src = false -> o = inl ol)
+      (TR: f_src = true -> o = inr or)
+      o1 (GENO: geno _ _ RR true f_tgt r_ctx (inr o1, itr_src) itr_tgt (ths, im_src, im_tgt, st_src, st_tgt, r_shared))
     :
-    __geno tid geno _geno RR f_src f_tgt r_ctx (o, Tau itr_src) itr_tgt (ths, im_src, im_tgt, st_src, st_tgt, r_shared)
+    _geno tid geno RR f_src f_tgt r_ctx (o, Tau itr_src) itr_tgt (ths, im_src, im_tgt, st_src, st_tgt, r_shared)
   | geno_chooseL
       f_src f_tgt r_ctx o
       ths im_src im_tgt st_src st_tgt r_shared
       X ktr_src itr_tgt
-      (GENO: exists x, _geno _ _ RR true f_tgt r_ctx (o, ktr_src x) itr_tgt (ths, im_src, im_tgt, st_src, st_tgt, r_shared))
+      ol or
+      (FL: f_src = false -> o = inl ol)
+      (TR: f_src = true -> o = inr or)
+      o1 (GENO: exists x, geno _ _ RR true f_tgt r_ctx (inr o1, ktr_src x) itr_tgt (ths, im_src, im_tgt, st_src, st_tgt, r_shared))
     :
-    __geno tid geno _geno RR f_src f_tgt r_ctx (o, trigger (Choose X) >>= ktr_src) itr_tgt (ths, im_src, im_tgt, st_src, st_tgt, r_shared)
+    _geno tid geno RR f_src f_tgt r_ctx (o, trigger (Choose X) >>= ktr_src) itr_tgt (ths, im_src, im_tgt, st_src, st_tgt, r_shared)
   | geno_putL
       f_src f_tgt r_ctx o
       ths im_src im_tgt st_src st_tgt r_shared
       st ktr_src itr_tgt
-      (GENO: _geno _ _ RR true f_tgt r_ctx (o, ktr_src tt) itr_tgt (ths, im_src, im_tgt, st, st_tgt, r_shared))
+      ol or
+      (FL: f_src = false -> o = inl ol)
+      (TR: f_src = true -> o = inr or)
+      o1 (GENO: geno _ _ RR true f_tgt r_ctx (inr o1, ktr_src tt) itr_tgt (ths, im_src, im_tgt, st, st_tgt, r_shared))
     :
-    __geno tid geno _geno RR f_src f_tgt r_ctx (o, trigger (Put st) >>= ktr_src) itr_tgt (ths, im_src, im_tgt, st_src, st_tgt, r_shared)
+    _geno tid geno RR f_src f_tgt r_ctx (o, trigger (Put st) >>= ktr_src) itr_tgt (ths, im_src, im_tgt, st_src, st_tgt, r_shared)
   | geno_getL
       f_src f_tgt r_ctx o
       ths im_src im_tgt st_src st_tgt r_shared
       ktr_src itr_tgt
-      (GENO: _geno _ _ RR true f_tgt r_ctx (o, ktr_src st_src) itr_tgt (ths, im_src, im_tgt, st_src, st_tgt, r_shared))
+      ol or
+      (FL: f_src = false -> o = inl ol)
+      (TR: f_src = true -> o = inr or)
+      o1 (GENO: geno _ _ RR true f_tgt r_ctx (inr o1, ktr_src st_src) itr_tgt (ths, im_src, im_tgt, st_src, st_tgt, r_shared))
     :
-    __geno tid geno _geno RR f_src f_tgt r_ctx (o, trigger (@Get _) >>= ktr_src) itr_tgt (ths, im_src, im_tgt, st_src, st_tgt, r_shared)
+    _geno tid geno RR f_src f_tgt r_ctx (o, trigger (@Get _) >>= ktr_src) itr_tgt (ths, im_src, im_tgt, st_src, st_tgt, r_shared)
   | geno_tidL
       f_src f_tgt r_ctx o
       ths im_src im_tgt st_src st_tgt r_shared
       ktr_src itr_tgt
-      (GENO: _geno _ _ RR true f_tgt r_ctx (o, ktr_src tid) itr_tgt (ths, im_src, im_tgt, st_src, st_tgt, r_shared))
+      ol or
+      (FL: f_src = false -> o = inl ol)
+      (TR: f_src = true -> o = inr or)
+      o1 (GENO: geno _ _ RR true f_tgt r_ctx (inr o1, ktr_src tid) itr_tgt (ths, im_src, im_tgt, st_src, st_tgt, r_shared))
     :
-    __geno tid geno _geno RR f_src f_tgt r_ctx (o, trigger (GetTid) >>= ktr_src) itr_tgt (ths, im_src, im_tgt, st_src, st_tgt, r_shared)
+    _geno tid geno RR f_src f_tgt r_ctx (o, trigger (GetTid) >>= ktr_src) itr_tgt (ths, im_src, im_tgt, st_src, st_tgt, r_shared)
   | geno_UB
       f_src f_tgt r_ctx o
       ths im_src im_tgt st_src st_tgt r_shared
       ktr_src itr_tgt
+      ol or
+      (FL: f_src = false -> o = inl ol)
+      (TR: f_src = true -> o = inr or)
     :
-    __geno tid geno _geno RR f_src f_tgt r_ctx (o, trigger (Undefined) >>= ktr_src) itr_tgt (ths, im_src, im_tgt, st_src, st_tgt, r_shared)
+    _geno tid geno RR f_src f_tgt r_ctx (o, trigger (Undefined) >>= ktr_src) itr_tgt (ths, im_src, im_tgt, st_src, st_tgt, r_shared)
   | geno_fairL
       f_src f_tgt r_ctx o
       ths im_src0 im_tgt st_src st_tgt r_shared
       f ktr_src itr_tgt
-      (GENO: exists im_src1,
-          (<<FAIR: fair_update im_src0 im_src1 (sum_fmap_r f)>>) /\
-            (<<GENO: _geno _ _ RR true f_tgt r_ctx (o, ktr_src tt) itr_tgt (ths, im_src1, im_tgt, st_src, st_tgt, r_shared)>>))
+      ol or
+      (FL: f_src = false -> o = inl ol)
+      (TR: f_src = true -> o = inr or)
+      o1 (GENO: exists im_src1,
+             (<<FAIR: fair_update im_src0 im_src1 (sum_fmap_r f)>>) /\
+               (<<GENO: geno _ _ RR true f_tgt r_ctx (inr o1, ktr_src tt) itr_tgt (ths, im_src1, im_tgt, st_src, st_tgt, r_shared)>>))
     :
-    __geno tid geno _geno RR f_src f_tgt r_ctx (o, trigger (Fair f) >>= ktr_src) itr_tgt (ths, im_src0, im_tgt, st_src, st_tgt, r_shared)
+    _geno tid geno RR f_src f_tgt r_ctx (o, trigger (Fair f) >>= ktr_src) itr_tgt (ths, im_src0, im_tgt, st_src, st_tgt, r_shared)
 
   | geno_tauR
       f_src f_tgt r_ctx o
       ths im_src im_tgt st_src st_tgt r_shared
       itr_src itr_tgt
-      (GENO: _geno _ _ RR f_src true r_ctx (o, itr_src) itr_tgt (ths, im_src, im_tgt, st_src, st_tgt, r_shared))
+      ol or
+      (FL: f_src = false -> o = inl ol)
+      (TR: f_src = true -> o = inr or)
+      (GENO: geno _ _ RR f_src true r_ctx (o, itr_src) itr_tgt (ths, im_src, im_tgt, st_src, st_tgt, r_shared))
     :
-    __geno tid geno _geno RR f_src f_tgt r_ctx (o, itr_src) (Tau itr_tgt) (ths, im_src, im_tgt, st_src, st_tgt, r_shared)
+    _geno tid geno RR f_src f_tgt r_ctx (o, itr_src) (Tau itr_tgt) (ths, im_src, im_tgt, st_src, st_tgt, r_shared)
   | geno_chooseR
       f_src f_tgt r_ctx o
       ths im_src im_tgt st_src st_tgt r_shared
       X itr_src ktr_tgt
-      (GENO: forall x, _geno _ _ RR f_src true r_ctx (o, itr_src) (ktr_tgt x) (ths, im_src, im_tgt, st_src, st_tgt, r_shared))
+      ol or
+      (FL: f_src = false -> o = inl ol)
+      (TR: f_src = true -> o = inr or)
+      (GENO: forall x, geno _ _ RR f_src true r_ctx (o, itr_src) (ktr_tgt x) (ths, im_src, im_tgt, st_src, st_tgt, r_shared))
     :
-    __geno tid geno _geno RR f_src f_tgt r_ctx (o, itr_src) (trigger (Choose X) >>= ktr_tgt) (ths, im_src, im_tgt, st_src, st_tgt, r_shared)
+    _geno tid geno RR f_src f_tgt r_ctx (o, itr_src) (trigger (Choose X) >>= ktr_tgt) (ths, im_src, im_tgt, st_src, st_tgt, r_shared)
   | geno_putR
       f_src f_tgt r_ctx o
       ths im_src im_tgt st_src st_tgt r_shared
       st itr_src ktr_tgt
-      (GENO: _geno _ _ RR f_src true r_ctx (o, itr_src) (ktr_tgt tt) (ths, im_src, im_tgt, st_src, st, r_shared))
+      ol or
+      (FL: f_src = false -> o = inl ol)
+      (TR: f_src = true -> o = inr or)
+      (GENO: geno _ _ RR f_src true r_ctx (o, itr_src) (ktr_tgt tt) (ths, im_src, im_tgt, st_src, st, r_shared))
     :
-    __geno tid geno _geno RR f_src f_tgt r_ctx (o, itr_src) (trigger (Put st) >>= ktr_tgt) (ths, im_src, im_tgt, st_src, st_tgt, r_shared)
+    _geno tid geno RR f_src f_tgt r_ctx (o, itr_src) (trigger (Put st) >>= ktr_tgt) (ths, im_src, im_tgt, st_src, st_tgt, r_shared)
   | geno_getR
       f_src f_tgt r_ctx o
       ths im_src im_tgt st_src st_tgt r_shared
       itr_src ktr_tgt
-      (GENO: _geno _ _ RR f_src true r_ctx (o, itr_src) (ktr_tgt st_tgt) (ths, im_src, im_tgt, st_src, st_tgt, r_shared))
+      ol or
+      (FL: f_src = false -> o = inl ol)
+      (TR: f_src = true -> o = inr or)
+      (GENO: geno _ _ RR f_src true r_ctx (o, itr_src) (ktr_tgt st_tgt) (ths, im_src, im_tgt, st_src, st_tgt, r_shared))
     :
-    __geno tid geno _geno RR f_src f_tgt r_ctx (o, itr_src) (trigger (@Get _) >>= ktr_tgt) (ths, im_src, im_tgt, st_src, st_tgt, r_shared)
+    _geno tid geno RR f_src f_tgt r_ctx (o, itr_src) (trigger (@Get _) >>= ktr_tgt) (ths, im_src, im_tgt, st_src, st_tgt, r_shared)
   | geno_tidR
       f_src f_tgt r_ctx o
       ths im_src im_tgt st_src st_tgt r_shared
       itr_src ktr_tgt
-      (GENO: _geno _ _ RR f_src true r_ctx (o, itr_src) (ktr_tgt tid) (ths, im_src, im_tgt, st_src, st_tgt, r_shared))
+      ol or
+      (FL: f_src = false -> o = inl ol)
+      (TR: f_src = true -> o = inr or)
+      (GENO: geno _ _ RR f_src true r_ctx (o, itr_src) (ktr_tgt tid) (ths, im_src, im_tgt, st_src, st_tgt, r_shared))
     :
-    __geno tid geno _geno RR f_src f_tgt r_ctx (o, itr_src) (trigger (GetTid) >>= ktr_tgt) (ths, im_src, im_tgt, st_src, st_tgt, r_shared)
+    _geno tid geno RR f_src f_tgt r_ctx (o, itr_src) (trigger (GetTid) >>= ktr_tgt) (ths, im_src, im_tgt, st_src, st_tgt, r_shared)
   | geno_fairR
       f_src f_tgt r_ctx o
       ths im_src im_tgt0 st_src st_tgt r_shared
       f itr_src ktr_tgt
+      ol or
+      (FL: f_src = false -> o = inl ol)
+      (TR: f_src = true -> o = inr or)
       (GENO: forall im_tgt1
                    (FAIR: fair_update im_tgt0 im_tgt1 (sum_fmap_r f)),
-          (<<GENO: _geno _ _ RR f_src true r_ctx (o, itr_src) (ktr_tgt tt) (ths, im_src, im_tgt1, st_src, st_tgt, r_shared)>>))
+          (<<GENO: geno _ _ RR f_src true r_ctx (o, itr_src) (ktr_tgt tt) (ths, im_src, im_tgt1, st_src, st_tgt, r_shared)>>))
     :
-    __geno tid geno _geno RR f_src f_tgt r_ctx (o, itr_src) (trigger (Fair f) >>= ktr_tgt) (ths, im_src, im_tgt0, st_src, st_tgt, r_shared)
+    _geno tid geno RR f_src f_tgt r_ctx (o, itr_src) (trigger (Fair f) >>= ktr_tgt) (ths, im_src, im_tgt0, st_src, st_tgt, r_shared)
 
   | geno_observe
       f_src f_tgt r_ctx o
       ths im_src im_tgt st_src st_tgt r_shared
       fn args ktr_src ktr_tgt
-      (GENO: forall ret,
-          _geno _ _ RR true true r_ctx (o, ktr_src ret) (ktr_tgt ret) (ths, im_src, im_tgt, st_src, st_tgt, r_shared))
+      ol or
+      (FL: f_src = false -> o = inl ol)
+      (TR: f_src = true -> o = inr or)
+      o1 (GENO: forall ret,
+             geno _ _ RR true true r_ctx (inr o1, ktr_src ret) (ktr_tgt ret) (ths, im_src, im_tgt, st_src, st_tgt, r_shared))
     :
-    __geno tid geno _geno RR f_src f_tgt r_ctx (o, trigger (Observe fn args) >>= ktr_src) (trigger (Observe fn args) >>= ktr_tgt) (ths, im_src, im_tgt, st_src, st_tgt, r_shared)
+    _geno tid geno RR f_src f_tgt r_ctx (o, trigger (Observe fn args) >>= ktr_src) (trigger (Observe fn args) >>= ktr_tgt) (ths, im_src, im_tgt, st_src, st_tgt, r_shared)
 
   | geno_yieldR
       f_src f_tgt r_ctx0 o0
       ths0 im_src0 im_tgt0 st_src0 st_tgt0 r_shared0
       r_own r_shared
       ktr_src ktr_tgt
+      ol0 or0
+      (FL: f_src = false -> o0 = inl ol0)
+      (TR: f_src = true -> o0 = inr or0)
       (INV: I (ths0, im_src0, im_tgt0, st_src0, st_tgt0, r_shared))
       (VALID: URA.wf (r_shared ⋅ r_own ⋅ r_ctx0))
-      (GENO: forall ths1 im_src1 im_tgt1 st_src1 st_tgt1 r_shared1 r_ctx1
-               (INV: I (ths1, im_src1, im_tgt1, st_src1, st_tgt1, r_shared1))
-               (VALID: URA.wf (r_shared1 ⋅ r_own ⋅ r_ctx1))
-               im_tgt2
-               (TGT: fair_update im_tgt1 im_tgt2 (sum_fmap_l (tids_fmap tid ths1))),
-        exists o1,
-            (<<GENO: _geno _ _ RR f_src true r_ctx1 (o1, trigger (Yield) >>= ktr_src) (ktr_tgt tt) (ths1, im_src1, im_tgt2, st_src1, st_tgt1, r_shared1)>>) /\
-              (<<STUTTER: wf_stt.(lt) o1 o0>>))
+      (GENOF: (f_src = false) ->
+              forall ths1 im_src1 im_tgt1 st_src1 st_tgt1 r_shared1 r_ctx1
+                (INV: I (ths1, im_src1, im_tgt1, st_src1, st_tgt1, r_shared1))
+                (VALID: URA.wf (r_shared1 ⋅ r_own ⋅ r_ctx1))
+                im_tgt2
+                (TGT: fair_update im_tgt1 im_tgt2 (sum_fmap_l (tids_fmap tid ths1))),
+              exists ol1,
+                (<<GENO: geno _ _ RR f_src true r_ctx1 (inl ol1, trigger (Yield) >>= ktr_src) (ktr_tgt tt) (ths1, im_src1, im_tgt2, st_src1, st_tgt1, r_shared1)>>) /\
+                  (<<STUTTER: wf_ot.(lt) ol1 ol0>>))
+      (GENOT: (f_src = true) ->
+              forall ths1 im_src1 im_tgt1 st_src1 st_tgt1 r_shared1 r_ctx1
+                (INV: I (ths1, im_src1, im_tgt1, st_src1, st_tgt1, r_shared1))
+                (VALID: URA.wf (r_shared1 ⋅ r_own ⋅ r_ctx1))
+                im_tgt2
+                (TGT: fair_update im_tgt1 im_tgt2 (sum_fmap_l (tids_fmap tid ths1))),
+              exists or1,
+                (<<GENO: geno _ _ RR f_src true r_ctx1 (inr or1, trigger (Yield) >>= ktr_src) (ktr_tgt tt) (ths1, im_src1, im_tgt2, st_src1, st_tgt1, r_shared1)>>) /\
+                  (<<STUTTER: wf_ot.(lt) or1 or0>>))
     :
-    __geno tid geno _geno RR f_src f_tgt r_ctx0 (o0, trigger (Yield) >>= ktr_src) (trigger (Yield) >>= ktr_tgt) (ths0, im_src0, im_tgt0, st_src0, st_tgt0, r_shared0)
+    _geno tid geno RR f_src f_tgt r_ctx0 (o0, trigger (Yield) >>= ktr_src) (trigger (Yield) >>= ktr_tgt) (ths0, im_src0, im_tgt0, st_src0, st_tgt0, r_shared0)
+
   | geno_yieldL
       f_src f_tgt r_ctx o0
       ths im_src0 im_tgt st_src st_tgt r_shared
       ktr_src itr_tgt
+      ol0 or0
+      (FL: f_src = false -> o0 = inl ol0)
+      (TR: f_src = true -> o0 = inr or0)
       (GENO: exists im_src1 o1,
           (<<FAIR: fair_update im_src0 im_src1 (sum_fmap_l (tids_fmap tid ths))>>) /\
-            (<<GENO: _geno _ _ RR true f_tgt r_ctx (o1, ktr_src tt) itr_tgt (ths, im_src1, im_tgt, st_src, st_tgt, r_shared)>>))
+            (<<GENO: geno _ _ RR true f_tgt r_ctx (inr o1, ktr_src tt) itr_tgt (ths, im_src1, im_tgt, st_src, st_tgt, r_shared)>>))
     :
-    __geno tid geno _geno RR f_src f_tgt r_ctx (o0, trigger (Yield) >>= ktr_src) itr_tgt (ths, im_src0, im_tgt, st_src, st_tgt, r_shared)
+    _geno tid geno RR f_src f_tgt r_ctx (o0, trigger (Yield) >>= ktr_src) itr_tgt (ths, im_src0, im_tgt, st_src, st_tgt, r_shared)
 
   | geno_progress
       r_ctx o
@@ -200,326 +264,455 @@ Section GENORDER.
       itr_src itr_tgt
       (GENO: ModSimNoSync.lsim I tid RR false false r_ctx itr_src itr_tgt (ths, im_src, im_tgt, st_src, st_tgt, r_shared))
     :
-    __geno tid geno _geno RR true true r_ctx (o, itr_src) itr_tgt (ths, im_src, im_tgt, st_src, st_tgt, r_shared)
+    _geno tid geno RR true true r_ctx (inr o, itr_src) itr_tgt (ths, im_src, im_tgt, st_src, st_tgt, r_shared)
   .
 
-  Definition lsim (tid: thread_id)
+  Definition geno (tid: thread_id)
              R_src R_tgt (RR: R_src -> R_tgt -> URA.car -> shared_rel):
     bool -> bool -> URA.car -> (wf_stt.(T) * itree srcE R_src) -> itree tgtE R_tgt -> shared_rel :=
-    paco9 (fun r => pind9 (__lsim tid r) top9) bot9 R_src R_tgt RR.
+    pind9 (_geno tid) top9 R_src R_tgt RR.
 
-  Lemma __lsim_mon tid:
-    forall r r' (LE: r <9= r'), (__lsim tid r) <10= (__lsim tid r').
-  Proof.
-    ii. inv PR; try (econs; eauto; fail).
-    eapply lsim_yieldR; eauto. i. hexploit LSIM; eauto. i. des. esplits; eauto.
-  Qed.
-
-  Lemma _lsim_mon tid: forall r, monotone9 (__lsim tid r).
+  Lemma geno_mon tid: monotone9 (_geno tid).
   Proof.
     ii. inv IN; try (econs; eauto; fail).
     { des. econs; eauto. }
     { des. econs; eauto. }
-    { econs. i. eapply LE. eapply LSIM. eauto. }
-    (* { econs; eauto. i. specialize (LSIM _ _ _ _ _ _ _ INV0 VALID0 _ TGT). des. esplits; eauto. } *)
+    { econs; eauto. i. eapply LE. eapply GENO. eauto. }
+    { econs; eauto.
+      - clear GENOT. i. specialize (GENOF H _ _ _ _ _ _ _ INV0 VALID0 _ TGT). des. esplits; eauto.
+      - clear GENOF. i. specialize (GENOT H _ _ _ _ _ _ _ INV0 VALID0 _ TGT). des. esplits; eauto.
+    }
     { des. econs; esplits; eauto. }
   Qed.
 
-  Lemma lsim_mon tid: forall q, monotone9 (fun r => pind9 (__lsim tid r) q).
+  Local Hint Constructors _geno: core.
+  Local Hint Unfold geno: core.
+  Local Hint Resolve geno_mon: paco.
+
+  (* Properties *)
+  Lemma geno_sfalse_oright
+        tid R0 R1 (RR: R0 -> R1 -> URA.car -> shared_rel)
+        pt r_ctx src tgt shr o
+    :
+    ~ (geno tid RR false pt r_ctx (inr o, src) tgt shr).
   Proof.
-    ii. eapply pind9_mon_gen; eauto.
-    ii. eapply __lsim_mon; eauto.
+    intros GENO.
+    match goal with | GENO: geno _ _ ?_ps _ _ ?_osrc _ _ |- _ => remember _ps as ps; remember _osrc as osrc end.
+    move GENO before tid. revert_until GENO.
+    pattern R0, R1, RR, ps, pt, r_ctx, osrc, tgt, shr.
+    revert R0 R1 RR ps pt r_ctx osrc tgt shr GENO. apply pind9_acc.
+    intros rr DEC IH. clear DEC. intros R0 R1 RR ps pt r_ctx osrc tgt shr GENO.
+    i; clarify.
+    eapply pind9_unfold in GENO; eauto with paco.
+    inv GENO; try (hexploit FL; ss; fail).
   Qed.
 
-  Variant lsim_resetC
-          (r: forall R_src R_tgt (RR: R_src -> R_tgt -> URA.car -> shared_rel), bool -> bool -> URA.car -> (wf_stt.(T) * itree srcE R_src) -> itree tgtE R_tgt -> shared_rel)
-          R_src R_tgt (RR: R_src -> R_tgt -> URA.car -> shared_rel)
+  Lemma geno_strue_oleft
+        tid R0 R1 (RR: R0 -> R1 -> URA.car -> shared_rel)
+        pt r_ctx src tgt shr o
     :
-    bool -> bool -> URA.car -> (wf_stt.(T) * itree srcE R_src) -> itree tgtE R_tgt -> shared_rel :=
-    | lsim_resetC_intro
-        src tgt shr r_ctx
-        ps0 pt0 ps1 pt1
-        (REL: r _ _ RR ps1 pt1 r_ctx src tgt shr)
-        (SRC: ps1 = true -> ps0 = true)
-        (TGT: pt1 = true -> pt0 = true)
-      :
-      lsim_resetC r RR ps0 pt0 r_ctx src tgt shr
-  .
-
-  Lemma lsim_resetC_spec tid
-    :
-    lsim_resetC <10= gupaco9 (fun r => pind9 (__lsim tid r) top9) (cpn9 (fun r => pind9 (__lsim tid r) top9)).
+    ~ (geno tid RR true pt r_ctx (inl o, src) tgt shr).
   Proof.
-    eapply wrespect9_uclo; eauto with paco.
-    { eapply lsim_mon. }
-    econs.
-    { ii. inv IN. econs; eauto. }
-    i. inv PR. eapply GF in REL.
-    eapply pind9_acc in REL.
-    instantiate (1:= (fun R0 R1 (RR: R0 -> R1 -> URA.car -> shared_rel) ps1 pt1 r_ctx src tgt shr =>
-                        forall ps0 pt0,
-                          (ps1 = true -> ps0 = true) ->
-                          (pt1 = true -> pt0 = true) ->
-                          pind9 (__lsim tid (rclo9 lsim_resetC r)) top9 R0 R1 RR ps0 pt0 r_ctx src tgt shr)) in REL; eauto.
-    ss. i. eapply pind9_unfold in PR.
-    2:{ eapply _lsim_mon. }
-    rename PR into LSIM. inv LSIM.
-
-    { eapply pind9_fold. econs; eauto. }
-
-    { destruct LSIM0 as [LSIM0 IND]. clear LSIM0.
-      eapply pind9_fold. eapply lsim_tauL. split; ss.
-      hexploit IH; eauto.
-    }
-
-    { des. eapply pind9_fold. eapply lsim_chooseL. esplits; eauto. split; ss.
-      destruct LSIM0 as [LSIM0 IND]. hexploit IH; eauto.
-    }
-
-    { eapply pind9_fold. eapply lsim_putL. split; ss.
-      destruct LSIM0 as [LSIM0 IND]. hexploit IH; eauto.
-    }
-
-    { eapply pind9_fold. eapply lsim_getL. split; ss.
-      destruct LSIM0 as [LSIM0 IND]. hexploit IH; eauto.
-    }
-
-    { eapply pind9_fold. eapply lsim_tidL. split; ss.
-      destruct LSIM0 as [LSIM0 IND]. hexploit IH; eauto.
-    }
-
-    { eapply pind9_fold. eapply lsim_UB. }
-
-    { des. eapply pind9_fold. eapply lsim_fairL. esplits; eauto. split; ss.
-      destruct LSIM as [LSIM IND]. hexploit IH; eauto.
-    }
-
-    { destruct LSIM0 as [LSIM0 IND]. clear LSIM0.
-      eapply pind9_fold. eapply lsim_tauR. split; ss.
-      hexploit IH. eauto. all: eauto.
-    }
-
-    { eapply pind9_fold. eapply lsim_chooseR. i. split; ss. specialize (LSIM0 x).
-      destruct LSIM0 as [LSIM0 IND]. hexploit IH; eauto.
-    }
-
-    { eapply pind9_fold. eapply lsim_putR. split; ss.
-      destruct LSIM0 as [LSIM0 IND]. hexploit IH; eauto.
-    }
-
-    { eapply pind9_fold. eapply lsim_getR. split; ss.
-      destruct LSIM0 as [LSIM0 IND]. hexploit IH; eauto.
-    }
-
-    { eapply pind9_fold. eapply lsim_tidR. split; ss.
-      destruct LSIM0 as [LSIM0 IND]. hexploit IH; eauto.
-    }
-
-    { eapply pind9_fold. eapply lsim_fairR. i. split; ss. specialize (LSIM0 _ FAIR).
-      des. destruct LSIM0 as [LSIM0 IND]. hexploit IH; eauto.
-    }
-
-    { eapply pind9_fold. eapply lsim_observe. i. eapply rclo9_base. auto. }
-
-    { eapply pind9_fold. eapply lsim_yieldR; eauto. i.
-      hexploit LSIM0; eauto. clear LSIM0. intros LSIM0. des. esplits; eauto.
-      eapply rclo9_base. auto.
-    }
-
-    { des. eapply pind9_fold. eapply lsim_yieldL. esplits; eauto. split; ss.
-      destruct LSIM as [LSIM IND]. hexploit IH; eauto.
-    }
-
-    { hexploit H; ss; i. hexploit H0; ss; i. clarify.
-      eapply pind9_fold. eapply lsim_progress. eapply rclo9_base; auto. }
+    intros GENO.
+    match goal with | GENO: geno _ _ ?_ps _ _ ?_osrc _ _ |- _ => remember _ps as ps; remember _osrc as osrc end.
+    move GENO before tid. revert_until GENO.
+    pattern R0, R1, RR, ps, pt, r_ctx, osrc, tgt, shr.
+    revert R0 R1 RR ps pt r_ctx osrc tgt shr GENO. apply pind9_acc.
+    intros rr DEC IH. clear DEC. intros R0 R1 RR ps pt r_ctx osrc tgt shr GENO.
+    i; clarify.
+    eapply pind9_unfold in GENO; eauto with paco.
+    inv GENO; try (hexploit TR; ss; fail).
   Qed.
 
-  Lemma lsim_reset_prog
-        tid
-        R0 R1 (RR: R0 -> R1 -> URA.car -> shared_rel)
-        src tgt shr
-        ps0 pt0 ps1 pt1 r_ctx
-        (LSIM: lsim tid RR ps1 pt1 r_ctx src tgt shr)
-        (SRC: ps1 = true -> ps0 = true)
-        (TGT: pt1 = true -> pt0 = true)
+  Lemma geno_ord_weak_left
+        tid R0 R1 (LRR: R0 -> R1 -> URA.car -> shared_rel)
+        ps pt r_ctx src tgt (shr: shared) o0 o1
+        (LT: wf_ot.(lt) o0 o1)
+        (GENO: geno tid LRR ps pt r_ctx (inl o0, src) tgt shr)
     :
-    lsim tid RR ps0 pt0 r_ctx src tgt shr.
+    geno tid LRR ps pt r_ctx (inl o1, src) tgt shr.
   Proof.
-    ginit.
-    { eapply lsim_mon. }
-    { eapply cpn9_wcompat. eapply lsim_mon. }
-    guclo lsim_resetC_spec.
-    { eapply lsim_mon. }
-    econs; eauto. gfinal.
-    { eapply lsim_mon. }
-    right. auto.
+    remember (inl o0, src) as osrc.
+    move GENO before tid. revert_until GENO.
+    pattern R0, R1, LRR, ps, pt, r_ctx, osrc, tgt, shr.
+    revert R0 R1 LRR ps pt r_ctx osrc tgt shr GENO. apply pind9_acc.
+    intros rr DEC IH. clear DEC. intros R0 R1 LRR ps pt r_ctx osrc tgt shr GENO.
+    i; clarify.
+    eapply pind9_unfold in GENO; eauto with paco.
+    inv GENO.
+
+    { eapply pind9_fold. econs 1; eauto. i. apply TR in H; ss. }
+    { eapply pind9_fold. econs 2; eauto. i. apply TR in H; ss.
+      eapply upind9_mon; eauto. ss.
+      Unshelve. exact o2.
+    }
+    { eapply pind9_fold. econs 3; eauto. i. apply TR in H; ss.
+      des. exists x.
+      eapply upind9_mon; eauto. ss.
+      Unshelve. exact o2.
+    }
+    { eapply pind9_fold. econs 4; eauto. i. apply TR in H; ss.
+      eapply upind9_mon; eauto. ss.
+      Unshelve. exact o2.
+    }
+    { eapply pind9_fold. econs 5; eauto. i. apply TR in H; ss.
+      eapply upind9_mon; eauto. ss.
+      Unshelve. exact o2.
+    }
+    { eapply pind9_fold. econs 6; eauto. i. apply TR in H; ss.
+      eapply upind9_mon; eauto. ss.
+      Unshelve. exact o2.
+    }
+    { eapply pind9_fold. econs 7; eauto. i. apply TR in H; ss.
+      Unshelve. exact o0.
+    }
+    { eapply pind9_fold. econs 8; eauto. i. apply TR in H; ss.
+      des. esplits; eauto.
+      eapply upind9_mon; eauto. ss.
+      Unshelve. exact o2.
+    }
+
+    { eapply pind9_fold. econs 9; eauto. i. apply TR in H; ss.
+      split; ss. destruct GENO0 as [GENO IND]. eapply IH in IND; eauto.
+      Unshelve. exact o1.
+    }
+    { eapply pind9_fold. econs 10; eauto. i. apply TR in H; ss.
+      i. specialize (GENO0 x).
+      split; ss. destruct GENO0 as [GENO IND]. eapply IH in IND; eauto.
+      Unshelve. exact o1.
+    }
+    { eapply pind9_fold. econs 11; eauto. i. apply TR in H; ss.
+      split; ss. destruct GENO0 as [GENO IND]. eapply IH in IND; eauto.
+      Unshelve. exact o1.
+    }
+    { eapply pind9_fold. econs 12; eauto. i. apply TR in H; ss.
+      split; ss. destruct GENO0 as [GENO IND]. eapply IH in IND; eauto.
+      Unshelve. exact o1.
+    }
+    { eapply pind9_fold. econs 13; eauto. i. apply TR in H; ss.
+      split; ss. destruct GENO0 as [GENO IND]. eapply IH in IND; eauto.
+      Unshelve. exact o1.
+    }
+    { eapply pind9_fold. econs 14; eauto. i. apply TR in H; ss.
+      i. specialize (GENO0 _ FAIR).
+      split; ss. destruct GENO0 as [GENO IND]. eapply IH in IND; eauto.
+      Unshelve. exact o1.
+    }
+    { eapply pind9_fold. econs 15; eauto. i. apply TR in H; ss.
+      i. specialize (GENO0 ret).
+      eapply upind9_mon; eauto. ss.
+      Unshelve. exact o2.
+    }
+
+    { eapply pind9_fold. econs 16; eauto. i. apply TR in H; ss.
+      - i. clear GENOT. specialize (GENOF H _ _ _ _ _ _ _ INV0 VALID0 _ TGT).
+        des. esplits; eauto.
+        split; ss. destruct GENO as [GENO IND]. eapply IH in IND; eauto.
+        apply FL in H. clarify.
+        Unshelve. exact o1.
+      - i. clear GENOF. apply TR in H; ss.
+    }
+
+    { eapply pind9_fold. econs 17; eauto. i. apply TR in H; ss.
+      des. esplits; eauto. destruct GENO as [GENO IND].
+      eapply upind9_mon; eauto. ss.
+      Unshelve. exact o1.
+    }
+
   Qed.
 
-  Lemma lsim_set_prog
-        tid
-        R0 R1 (RR: R0 -> R1 -> URA.car -> shared_rel)
-        r_ctx src tgt shr
-        (LSIM: lsim tid RR true true r_ctx src tgt shr)
+  Lemma geno_ord_weak_right
+        tid R0 R1 (LRR: R0 -> R1 -> URA.car -> shared_rel)
+        ps pt r_ctx src tgt (shr: shared) o0 o1
+        (LT: wf_ot.(lt) o0 o1)
+        (GENO: geno tid LRR ps pt r_ctx (inr o0, src) tgt shr)
     :
-    forall ps pt, lsim tid RR ps pt r_ctx src tgt shr.
+    geno tid LRR ps pt r_ctx (inr o1, src) tgt shr.
   Proof.
-    i. revert_until tid. pcofix CIH. i.
-    remember true as ps0 in LSIM at 1. remember true as pt0 in LSIM at 1.
-    move LSIM before CIH. revert_until LSIM. punfold LSIM.
-    2:{ eapply lsim_mon. }
-    eapply pind9_acc in LSIM.
+    remember (inr o0, src) as osrc.
+    move GENO before tid. revert_until GENO.
+    pattern R0, R1, LRR, ps, pt, r_ctx, osrc, tgt, shr.
+    revert R0 R1 LRR ps pt r_ctx osrc tgt shr GENO. apply pind9_acc.
+    intros rr DEC IH. clear DEC. intros R0 R1 LRR ps pt r_ctx osrc tgt shr GENO.
+    i; clarify.
+    eapply pind9_unfold in GENO; eauto with paco.
+    inv GENO.
 
-    { instantiate (1:= (fun R0 R1 (RR: R0 -> R1 -> URA.car -> shared_rel) ps0 pt0 r_ctx src tgt shr =>
-                          ps0 = true ->
-                          pt0 = true ->
-                          forall ps pt,
-                            paco9
-                              (fun r0 =>
-                                 pind9 (__lsim tid r0) top9) r R0 R1 RR ps pt r_ctx src tgt shr)) in LSIM; auto. }
+    { eapply pind9_fold. econs 1; eauto. i. apply FL in H; ss. }
+    { eapply pind9_fold. econs 2; eauto. i. apply FL in H; ss.
+      eapply upind9_mon; eauto. ss.
+      Unshelve. exact o2.
+    }
+    { eapply pind9_fold. econs 3; eauto. i. apply FL in H; ss.
+      des. exists x.
+      eapply upind9_mon; eauto. ss.
+      Unshelve. exact o2.
+    }
+    { eapply pind9_fold. econs 4; eauto. i. apply FL in H; ss.
+      eapply upind9_mon; eauto. ss.
+      Unshelve. exact o2.
+    }
+    { eapply pind9_fold. econs 5; eauto. i. apply FL in H; ss.
+      eapply upind9_mon; eauto. ss.
+      Unshelve. exact o2.
+    }
+    { eapply pind9_fold. econs 6; eauto. i. apply FL in H; ss.
+      eapply upind9_mon; eauto. ss.
+      Unshelve. exact o2.
+    }
+    { eapply pind9_fold. econs 7; eauto. i. apply FL in H; ss.
+      Unshelve. exact o0.
+    }
+    { eapply pind9_fold. econs 8; eauto. i. apply FL in H; ss.
+      des. esplits; eauto.
+      eapply upind9_mon; eauto. ss.
+      Unshelve. exact o2.
+    }
 
-    ss. clear ps0 pt0 r_ctx src tgt shr LSIM.
-    intros rr DEC IH R0' R1' RR' gps gpt r_ctx src tgt shr LSIM. clear DEC.
-    intros Egps Egpt ps pt.
-    eapply pind9_unfold in LSIM.
-    2:{ eapply _lsim_mon. }
+    { eapply pind9_fold. econs 9; eauto. i. apply FL in H; ss.
+      split; ss. destruct GENO0 as [GENO IND]. eapply IH in IND; eauto.
+      Unshelve. exact o1.
+    }
+    { eapply pind9_fold. econs 10; eauto. i. apply FL in H; ss.
+      i. specialize (GENO0 x).
+      split; ss. destruct GENO0 as [GENO IND]. eapply IH in IND; eauto.
+      Unshelve. exact o1.
+    }
+    { eapply pind9_fold. econs 11; eauto. i. apply FL in H; ss.
+      split; ss. destruct GENO0 as [GENO IND]. eapply IH in IND; eauto.
+      Unshelve. exact o1.
+    }
+    { eapply pind9_fold. econs 12; eauto. i. apply FL in H; ss.
+      split; ss. destruct GENO0 as [GENO IND]. eapply IH in IND; eauto.
+      Unshelve. exact o1.
+    }
+    { eapply pind9_fold. econs 13; eauto. i. apply FL in H; ss.
+      split; ss. destruct GENO0 as [GENO IND]. eapply IH in IND; eauto.
+      Unshelve. exact o1.
+    }
+    { eapply pind9_fold. econs 14; eauto. i. apply FL in H; ss.
+      i. specialize (GENO0 _ FAIR).
+      split; ss. destruct GENO0 as [GENO IND]. eapply IH in IND; eauto.
+      Unshelve. exact o1.
+    }
+    { eapply pind9_fold. econs 15; eauto. i. apply FL in H; ss.
+      i. specialize (GENO0 ret).
+      eapply upind9_mon; eauto. ss.
+      Unshelve. exact o2.
+    }
+
+    { eapply pind9_fold. econs 16; eauto. i. apply FL in H; ss.
+      - i. clear GENOT. apply FL in H; ss.
+      - i. clear GENOF. specialize (GENOT H _ _ _ _ _ _ _ INV0 VALID0 _ TGT).
+        des. esplits; eauto.
+        split; ss. destruct GENO as [GENO IND]. eapply IH in IND; eauto.
+        apply TR in H. clarify.
+        Unshelve. exact o1.
+    }
+
+    { eapply pind9_fold. econs 17; eauto. i. apply FL in H; ss.
+      des. esplits; eauto. destruct GENO as [GENO IND].
+      eapply upind9_mon; eauto. ss.
+      Unshelve. exact o1.
+    }
+
+    { eapply pind9_fold. econs 18; eauto. }
+
+  Qed.
+
+  Lemma nosync_geno
+        tid R0 R1 (RR: R0 -> R1 -> URA.car -> shared_rel)
+        ps pt r_ctx src tgt shr
+        (LSIM: ModSimNoSync.lsim I tid RR ps pt r_ctx src tgt shr)
+    :
+    exists o, geno tid RR ps pt r_ctx (o, src) tgt shr.
+  Proof.
+    punfold LSIM.
+    pattern R0, R1, RR, ps, pt, r_ctx, src, tgt, shr.
+    revert R0 R1 RR ps pt r_ctx src tgt shr LSIM. apply pind9_acc.
+    intros rr DEC IH. clear DEC. intros R0 R1 RR ps pt r_ctx src tgt shr LSIM.
+    eapply pind9_unfold in LSIM; eauto with paco.
+    (* specialize (one R0 R1). specialize (@fzero R0 R1). *)
+    set (fzero:= fun _: (A R0 R1) => @ord_tree_base (A R0 R1)). set (one:= ord_tree_cons fzero).
     inv LSIM.
 
-    { pfold. eapply pind9_fold. econs; eauto. }
-
-    { destruct LSIM0 as [LSIM0 IND]. clear LSIM0.
-      pfold. eapply pind9_fold. eapply lsim_tauL. split; ss.
-      hexploit IH. eauto. all: eauto. i. punfold H. eapply lsim_mon.
+    { exists (if ps then (inr one) else (inl one)).
+      eapply pind9_fold. econs 1; eauto. des_ifs. des_ifs.
+      1,2: instantiate (1:=fzero (ps, pt, r_ctx, Ret r_src, Ret r_tgt, (ths, im_src, im_tgt, st_src, st_tgt, r_shared))); ss.
     }
 
-    { des. pfold. eapply pind9_fold. eapply lsim_chooseL. esplits; eauto. split; ss.
-      destruct LSIM0 as [LSIM0 IND]. hexploit IH; eauto. i. punfold H. eapply lsim_mon.
+    { exists (if ps then (inr one) else (inl one)).
+      destruct LSIM0 as [LSIM IND]. eapply IH in IND. des.
+      destruct o. apply geno_strue_oleft in IND; ss.
+      eapply pind9_fold. econs 2; eauto. 1,2: des_ifs.
+      split; ss. eauto.
+    }
+    { exists (if ps then (inr one) else (inl one)).
+      des. destruct LSIM0 as [LSIM IND]. eapply IH in IND. des.
+      destruct o. apply geno_strue_oleft in IND; ss.
+      eapply pind9_fold. econs 3; eauto. 1,2: des_ifs.
+      eexists; split; ss. eauto.
+    }
+    { exists (if ps then (inr one) else (inl one)).
+      destruct LSIM0 as [LSIM IND]. eapply IH in IND. des.
+      destruct o. apply geno_strue_oleft in IND; ss.
+      eapply pind9_fold. econs 4; eauto. 1,2: des_ifs.
+      split; ss. eauto.
+    }
+    { exists (if ps then (inr one) else (inl one)).
+      destruct LSIM0 as [LSIM IND]. eapply IH in IND. des.
+      destruct o. apply geno_strue_oleft in IND; ss.
+      eapply pind9_fold. econs 5; eauto. 1,2: des_ifs.
+      split; ss. eauto.
+    }
+    { exists (if ps then (inr one) else (inl one)).
+      destruct LSIM0 as [LSIM IND]. eapply IH in IND. des.
+      destruct o. apply geno_strue_oleft in IND; ss.
+      eapply pind9_fold. econs 6; eauto. 1,2: des_ifs.
+      split; ss. eauto.
+    }
+    { exists (if ps then (inr one) else (inl one)).
+      eapply pind9_fold. econs 7; eauto. 1,2: des_ifs.
+    }
+    { exists (if ps then (inr one) else (inl one)).
+      des. destruct LSIM as [LSIM IND]. eapply IH in IND. des.
+      destruct o. apply geno_strue_oleft in IND; ss.
+      eapply pind9_fold. econs 8; eauto. 1,2: des_ifs.
+      esplits; eauto. split; ss. eauto.
     }
 
-    { pfold. eapply pind9_fold. eapply lsim_putL. split; ss.
-      destruct LSIM0 as [LSIM0 IND]. hexploit IH; eauto. i. punfold H. eapply lsim_mon.
+    { destruct LSIM0 as [LSIM IND]. eapply IH in IND. des. exists o.
+      destruct ps; destruct o.
+      1:{ apply geno_strue_oleft in IND; ss. }
+      3:{ apply geno_sfalse_oright in IND; ss. }
+      - eapply pind9_fold. econs 9; eauto. ss. split; ss; auto.
+      - eapply pind9_fold. econs 9; eauto. ss. split; ss; auto.
+        Unshelve. all: exact t.
     }
 
-    { pfold. eapply pind9_fold. eapply lsim_getL. split; ss.
-      destruct LSIM0 as [LSIM0 IND]. hexploit IH; eauto. i. punfold H. eapply lsim_mon.
+    { hexploit ord_tree_join.
+      { instantiate (2:=A R0 R1).
+        instantiate (2:= fun '(ps, pt, rs, src, tgt, shr) => @rr R0 R1 RR ps pt rs src tgt shr).
+        i. ss. des_ifs. eapply IH in SAT.
+        instantiate (1:= fun '(ps, pt, rs, src, tgt, shr) o =>
+                           geno tid RR ps pt rs (if ps then (inr o) else (inl o), src) tgt shr).
+        des. destruct b; destruct o.
+        1:{ apply geno_strue_oleft in SAT; ss. }
+        3:{ apply geno_sfalse_oright in SAT; ss. }
+        all: eauto.
+      }
+      intro JOIN. des. exists (if ps then (inr o1) else (inl o1)).
+      eapply pind9_fold. econs 10. 1,2: des_ifs.
+      i. specialize (LSIM0 x). destruct LSIM0 as [LSIM IND].
+      specialize (JOIN (ps, true, r_ctx, src, (ktr_tgt x), (ths, im_src, im_tgt, st_src, st_tgt, r_shared))).
+      destruct JOIN; auto. des. split; ss. des_ifs.
+      eapply geno_ord_weak_right; eauto.
+      eapply geno_ord_weak_left; eauto.
     }
 
-    { pfold. eapply pind9_fold. eapply lsim_tidL. split; ss.
-      destruct LSIM0 as [LSIM0 IND]. hexploit IH; eauto. i. punfold H. eapply lsim_mon.
+    { destruct LSIM0 as [LSIM IND]. eapply IH in IND. des. exists o.
+      destruct ps; destruct o.
+      1:{ apply geno_strue_oleft in IND; ss. }
+      3:{ apply geno_sfalse_oright in IND; ss. }
+      - eapply pind9_fold. econs 11; eauto. ss. split; ss; auto.
+      - eapply pind9_fold. econs 11; eauto. ss. split; ss; auto.
+        Unshelve. all: exact t.
+    }
+    { destruct LSIM0 as [LSIM IND]. eapply IH in IND. des. exists o.
+      destruct ps; destruct o.
+      1:{ apply geno_strue_oleft in IND; ss. }
+      3:{ apply geno_sfalse_oright in IND; ss. }
+      - eapply pind9_fold. econs 12; eauto. ss. split; ss; auto.
+      - eapply pind9_fold. econs 12; eauto. ss. split; ss; auto.
+        Unshelve. all: exact t.
+    }
+    { destruct LSIM0 as [LSIM IND]. eapply IH in IND. des. exists o.
+      destruct ps; destruct o.
+      1:{ apply geno_strue_oleft in IND; ss. }
+      3:{ apply geno_sfalse_oright in IND; ss. }
+      - eapply pind9_fold. econs 13; eauto. ss. split; ss; auto.
+      - eapply pind9_fold. econs 13; eauto. ss. split; ss; auto.
+        Unshelve. all: exact t.
     }
 
-    { pfold. eapply pind9_fold. eapply lsim_UB. }
-
-    { des. pfold. eapply pind9_fold. eapply lsim_fairL. esplits; eauto. split; ss.
-      destruct LSIM as [LSIM IND]. hexploit IH; eauto. i. punfold H. eapply lsim_mon.
+    { hexploit ord_tree_join.
+      { instantiate (2:=A R0 R1).
+        instantiate (2:= fun '(ps, pt, rs, src, tgt, shr) => @rr R0 R1 RR ps pt rs src tgt shr).
+        i. ss. des_ifs. eapply IH in SAT.
+        instantiate (1:= fun '(ps, pt, rs, src, tgt, shr) o =>
+                           geno tid RR ps pt rs (if ps then (inr o) else (inl o), src) tgt shr).
+        des. destruct b; destruct o.
+        1:{ apply geno_strue_oleft in SAT; ss. }
+        3:{ apply geno_sfalse_oright in SAT; ss. }
+        all: eauto.
+      }
+      intro JOIN. des. exists (if ps then (inr o1) else (inl o1)).
+      eapply pind9_fold. econs 14. 1,2: des_ifs.
+      i. specialize (LSIM0 _ FAIR). destruct LSIM0 as [LSIM IND].
+      specialize (JOIN (ps, true, r_ctx, src, (ktr_tgt ()), (ths, im_src, im_tgt1, st_src, st_tgt, r_shared))).
+      destruct JOIN; auto. des. split; ss. des_ifs.
+      eapply geno_ord_weak_right; eauto.
+      eapply geno_ord_weak_left; eauto.
     }
 
-    { destruct LSIM0 as [LSIM0 IND]. clear LSIM0.
-      pfold. eapply pind9_fold. eapply lsim_tauR. split; ss.
-      hexploit IH. eauto. all: eauto. i. punfold H. eapply lsim_mon.
+    { hexploit ord_tree_join.
+      { instantiate (2:=A R0 R1).
+        instantiate (2:= fun '(ps, pt, rs, src, tgt, shr) => @rr R0 R1 RR ps pt rs src tgt shr).
+        i. ss. des_ifs. eapply IH in SAT.
+        instantiate (1:= fun '(ps, pt, rs, src, tgt, shr) o =>
+                           geno tid RR ps pt rs (if ps then (inr o) else (inl o), src) tgt shr).
+        des. destruct b; destruct o.
+        1:{ apply geno_strue_oleft in SAT; ss. }
+        3:{ apply geno_sfalse_oright in SAT; ss. }
+        all: eauto.
+      }
+      intro JOIN. des. exists (if ps then (inr o1) else (inl o1)).
+      eapply pind9_fold. econs 15. 1,2: des_ifs.
+      i. specialize (LSIM0 ret). destruct LSIM0 as [LSIM IND].
+      specialize (JOIN (true, true, r_ctx, ktr_src ret, ktr_tgt ret, (ths, im_src, im_tgt, st_src, st_tgt, r_shared))).
+      destruct JOIN; auto. des. split; ss.
+      eapply geno_ord_weak_right; eauto.
     }
 
-    { pfold. eapply pind9_fold. eapply lsim_chooseR. i. split; ss. specialize (LSIM0 x).
-      destruct LSIM0 as [LSIM0 IND]. hexploit IH; eauto. i. punfold H. eapply lsim_mon.
+    { hexploit ord_tree_join.
+      { instantiate (2:=A R0 R1).
+        instantiate (2:= fun '(ps, pt, rs, src, tgt, shr) => @rr R0 R1 RR ps pt rs src tgt shr).
+        i. ss. des_ifs. eapply IH in SAT.
+        instantiate (1:= fun '(ps, pt, rs, src, tgt, shr) o =>
+                           geno tid RR ps pt rs (if ps then (inr o) else (inl o), src) tgt shr).
+        des. destruct b; destruct o.
+        1:{ apply geno_strue_oleft in SAT; ss. }
+        3:{ apply geno_sfalse_oright in SAT; ss. }
+        all: eauto.
+      }
+      intro JOIN. des. exists (if ps then (inr o1) else (inl o1)).
+      eapply pind9_fold. econs 16. 1,2: des_ifs.
+      1,2: eauto.
+      - i. specialize (LSIM0 _ _ _ _ _ _ _ INV0 VALID0 _ TGT). destruct LSIM0 as [LSIM IND].
+        specialize (JOIN (ps, true, r_ctx1, (x <- trigger Yield;; ktr_src x), ktr_tgt (), (ths1, im_src1, im_tgt2, st_src1, st_tgt1, r_shared1))).
+        destruct JOIN; auto. des. clarify. esplits; eauto. split; ss.
+      - i. specialize (LSIM0 _ _ _ _ _ _ _ INV0 VALID0 _ TGT). destruct LSIM0 as [LSIM IND].
+        specialize (JOIN (ps, true, r_ctx1, (x <- trigger Yield;; ktr_src x), ktr_tgt (), (ths1, im_src1, im_tgt2, st_src1, st_tgt1, r_shared1))).
+        destruct JOIN; auto. des. clarify. esplits; eauto. split; ss.
     }
 
-    { pfold. eapply pind9_fold. eapply lsim_putR. split; ss.
-      destruct LSIM0 as [LSIM0 IND]. hexploit IH; eauto. i. punfold H. eapply lsim_mon.
+    { des. destruct LSIM as [LSIM IND]. eapply IH in IND. des.
+      destruct o. apply geno_strue_oleft in IND; ss.
+      exists (if ps then (inr one) else (inl one)).
+      eapply pind9_fold. econs 17; eauto. 1,2: des_ifs. esplits; eauto.
+      split; ss. eauto.
     }
 
-    { pfold. eapply pind9_fold. eapply lsim_getR. split; ss.
-      destruct LSIM0 as [LSIM0 IND]. hexploit IH; eauto. i. punfold H. eapply lsim_mon.
-    }
-
-    { pfold. eapply pind9_fold. eapply lsim_tidR. split; ss.
-      destruct LSIM0 as [LSIM0 IND]. hexploit IH; eauto. i. punfold H. eapply lsim_mon.
-    }
-
-    { pfold. eapply pind9_fold. eapply lsim_fairR. i. split; ss. specialize (LSIM0 _ FAIR).
-      des. destruct LSIM0 as [LSIM0 IND]. hexploit IH; eauto. i. punfold H. eapply lsim_mon.
-    }
-
-    { pfold. eapply pind9_fold. eapply lsim_observe. i. eapply upaco9_mon_bot; eauto. }
-
-    { pfold. eapply pind9_fold. eapply lsim_yieldR; eauto. i.
-      hexploit LSIM0; eauto. clear LSIM0. intros LSIM0. des. esplits; eauto.
-      eapply upaco9_mon_bot; eauto.
-    }
-
-    { des. pfold. eapply pind9_fold. eapply lsim_yieldL. esplits; eauto. split; ss.
-      destruct LSIM as [LSIM IND]. hexploit IH; eauto. i. punfold H. eapply lsim_mon.
-    }
-
-    { pclearbot. eapply paco9_mon_bot. eapply lsim_reset_prog. eauto. all: ss. }
+    { exists (inr (@ord_tree_base _)). eapply pind9_fold. econs 18. pclearbot. auto. }
 
   Qed.
 
-  Definition local_RR {R0 R1} (RR: R0 -> R1 -> Prop) tid:
-    R0 -> R1 -> URA.car -> shared_rel :=
-    fun (r_src: R0) (r_tgt: R1) (r_ctx: URA.car) '(ths2, im_src1, im_tgt1, st_src1, st_tgt1, r_shared1) =>
-      (exists ths3 r_own r_shared2,
-          (<<THS: NatMap.remove tid ths2 = ths3>>) /\
-            (<<VALID: URA.wf (r_shared2 ⋅ r_own ⋅ r_ctx)>>) /\
-            (<<INV: I (ths3, im_src1, im_tgt1, st_src1, st_tgt1, r_shared2)>>) /\
-            (<<RET: RR r_src r_tgt>>)).
+  (*TODO: reduction lemmas*)
 
-  (* Definition local_RR {R0 R1} (RR: R0 -> R1 -> Prop) tid: *)
-  (*   R0 -> R1 -> URA.car -> wf_stt.(T) -> shared_rel := *)
-  (*   fun (r_src: R0) (r_tgt: R1) (r_ctx: URA.car) (o: wf_stt.(T)) '(ths2, im_src1, im_tgt1, st_src1, st_tgt1, r_shared1) => *)
-  (*     (exists ths3 r_own o0 r_shared2, *)
-  (*         (<<THS: NatMap.remove tid ths2 = ths3>>) /\ *)
-  (*           (<<VALID: URA.wf (r_shared2 ⋅ r_own ⋅ r_ctx)>>) /\ *)
-  (*           (<<INV: I (ths3, im_src1, im_tgt1, st_src1, st_tgt1, r_shared2)>>) /\ *)
-  (*           (<<STT: wf_stt.(lt) o0 o>>) /\ *)
-  (*           (<<RET: RR r_src r_tgt>>)). *)
-
-  (* Definition embed_lrr {R0 R1} (LRR: R0 -> R1 -> URA.car -> shared_rel): *)
-  (*   R0 -> R1 -> URA.car -> wf_stt.(T) -> shared_rel := *)
-  (*   fun (r_src: R0) (r_tgt: R1) (r_ctx: URA.car) (o: wf_stt.(T)) shr => *)
-  (*     (<<LSIM: LRR r_src r_tgt r_ctx shr>>) /\ (<<STT: exists o0, wf_stt.(lt) o0 o>>). *)
-
-  Definition local_sim {R0 R1} (RR: R0 -> R1 -> Prop) src tgt :=
-    forall ths0 im_src0 im_tgt0 st_src0 st_tgt0 r_shared0 r_ctx0
-      (INV: I (ths0, im_src0, im_tgt0, st_src0, st_tgt0, r_shared0))
-      tid ths1
-      (THS: TIdSet.add_new tid ths0 ths1)
-      (VALID: URA.wf (r_shared0 ⋅ r_ctx0)),
-    exists r_shared1 r_own,
-      (<<INV: I (ths1, im_src0, im_tgt0, st_src0, st_tgt0, r_shared1)>>) /\
-        (<<VALID: URA.wf (r_shared1 ⋅ r_own ⋅ r_ctx0)>>) /\
-        (forall ths im_src1 im_tgt1 st_src st_tgt r_shared2 r_ctx2
-           (INV: I (ths, im_src1, im_tgt1, st_src, st_tgt, r_shared2))
-           (VALID: URA.wf (r_shared2 ⋅ r_own ⋅ r_ctx2))
-           im_tgt2
-           (TGT: fair_update im_tgt1 im_tgt2 (sum_fmap_l (tids_fmap tid ths))),
-          exists o,
-          exists im_src2, (<<SRC: fair_update im_src1 im_src2 (sum_fmap_l (tids_fmap tid ths))>>) /\
-                       (<<LSIM: forall fs ft,
-                           lsim
-                             tid
-                             (@local_RR R0 R1 RR tid)
-                             fs ft
-                             r_ctx2
-                             (o, src) tgt
-                             (ths, im_src2, im_tgt2, st_src, st_tgt, r_shared2)
-                             >>)).
-
-  (* Definition shared_rel_wf: Prop := *)
-  (*   forall ths im_src0 im_tgt0 st_src st_tgt r_shared0 r_ctx *)
-  (*          (INV: I (ths, im_src0, im_tgt0, st_src, st_tgt, r_shared0)) *)
-  (*          (VALID: URA.wf (r_shared0 ⋅ r_ctx)), *)
-  (*   forall im_tgt1 *)
-  (*          (TGT: fair_update im_tgt0 im_tgt1 (sum_fmap_l (tids_fmap_all ths))), *)
-  (*   exists im_src1 r_shared1, *)
-  (*     (<<SRC: fair_update im_src0 im_src1 (sum_fmap_l (tids_fmap_all ths))>>) /\ *)
-  (*       (<<INV: I (ths, im_src1, im_tgt1, st_src, st_tgt, r_shared1)>>) /\ *)
-  (*       (<<VALID: URA.wf (r_shared1 ⋅ r_ctx)>>). *)
-
-End PRIMIVIESIM.
-#[export] Hint Constructors __lsim: core.
-#[export] Hint Unfold lsim: core.
-#[export] Hint Resolve __lsim_mon: paco.
-#[export] Hint Resolve _lsim_mon: paco.
-#[export] Hint Resolve lsim_mon: paco.
+End GENORDER.
+#[export] Hint Constructors _geno: core.
+#[export] Hint Unfold geno: core.
+#[export] Hint Resolve geno_mon: paco.
 
 Section PROOF.
 
