src/WFLib.v
@@ -254,3 +254,6 @@ Section WFTYPE.
 End WFTYPE.
 
 Definition ord_tree_WF {A}: WF := mk_wf (@ord_tree_lt_well_founded A).
+
+Definition sum_WF (A B: WF): WF := mk_wf (sum_lt_well_founded A.(wf) B.(wf)).
+Definition prod_WF (A B: WF): WF := mk_wf (prod_lt_well_founded A.(wf) B.(wf)).
